Update Treaps.thy

homework/Treaps.thy
@@ -38,8 +38,25 @@ fun set :: "('a::linorder) treap \<Rightarrow> ('a \<times> real) set" where
   Leaf: "set \<langle>\<rangle> = {}" |
   Node: "set \<langle>l, k, p, r\<rangle> = {(k, p)} \<union> set l \<union> set r"
 
-lemma set_finite: "finite (set t)"
-  by(induction t, auto)
+fun keys :: "('a::linorder) treap \<Rightarrow> 'a set" where
+  "keys \<langle>\<rangle> = {}" |
+  "keys \<langle>l, k, p, r\<rangle> = {k} \<union> keys l \<union> keys r"
+
+fun prios :: "('a::linorder) treap \<Rightarrow> real set" where
+  "prios \<langle>\<rangle> = {}" |
+  "prios \<langle>l, k, p, r\<rangle> = {p} \<union> prios l \<union> prios r"
+
+lemma set_finite: "finite (set t)" by(induction t, auto)
+lemma keys_finite: "finite (keys t)" by(induction t, auto)
+lemma prios_finite: "finite (prios t)" by(induction t, auto)
+
+inductive child_of :: "('a::linorder) treap \<Rightarrow> ('a::linorder) treap \<Rightarrow> bool" where
+  Left: "child_of l \<langle>l, k, p, r\<rangle>" |
+  Right: "child_of r \<langle>l, k, p, r\<rangle>" |
+  Cont: "\<lbrakk> child_of a b; child_of b c \<rbrakk> \<Longrightarrow> child_of a c"
+
+definition parent_of :: "('a::linorder) treap \<Rightarrow> ('a::linorder) treap \<Rightarrow> bool" where
+  "parent_of a b \<equiv> child_of b a"
 
 inductive distinct_keys :: "('a::linorder) treap \<Rightarrow> bool" where
   Leaf: "distinct_keys \<langle>\<rangle> " |
@@ -91,11 +108,17 @@ lemma distinct_root_key: "distinct_keys \<langle>l, k, p, r\<rangle> \<Longright
 lemma distinct_root: "is_distinct \<langle>l, k, p, r\<rangle> \<Longrightarrow> (k, p) \<notin> set l \<union> set r"
   using distinct_root_key is_distinct_def by blast
 
-lemma childs_disjoint_key: "distinct_keys \<langle>l, k, p, r\<rangle> \<Longrightarrow> set l \<inter> set r = {}"
+lemma child_dist_if_parent_dist:
+  assumes "child_of c p"
+      and "is_distinct p"
+    shows "is_distinct c"
+  using assms distinct_rev by(induction c p rule: child_of.induct, auto)
+
+lemma lrchilds_disjoint_key: "distinct_keys \<langle>l, k, p, r\<rangle> \<Longrightarrow> set l \<inter> set r = {}"
   by(induction "\<langle>l, k, p, r\<rangle>" arbitrary: k p rule: distinct_keys.induct, auto)
 
-lemma childs_disjoint: "is_distinct \<langle>l, k, p, r\<rangle> \<Longrightarrow> set l \<inter> set r = {}"
-  using childs_disjoint_key is_distinct_def by blast
+lemma lrchilds_disjoint: "is_distinct \<langle>l, k, p, r\<rangle> \<Longrightarrow> set l \<inter> set r = {}"
+  using lrchilds_disjoint_key is_distinct_def by blast
 
 lemma size_correct: "is_distinct t \<Longrightarrow> size t = card (set t)"
 proof(induction t)
@@ -111,7 +134,7 @@ proof(induction t)
   ultimately have "size \<langle>l, k, p, r\<rangle> = card (set l) + card (set r) + 1"
     by simp
   also have "... = card (set l \<union> set r) + 1"
-    using Node.prems childs_disjoint set_finite card_Un_disjoint
+    using Node.prems lrchilds_disjoint set_finite card_Un_disjoint
     by metis
   also have "... = card (set \<langle>l, k, p, r\<rangle> - {(k, p)}) + 1"
     using Node.prems distinct_root by fastforce
@@ -135,30 +158,48 @@ using assms proof(induction t rule: set.induct)
   then show ?case by simp
 qed(simp)
 
-lemma "set t \<noteq> {} \<Longrightarrow> is_distinct t \<Longrightarrow> card {(k', p') \<in> set t. k} = 1"
-  apply(induction t, auto) sledgehammer
-
 lemma pair_unique:
   assumes "is_distinct t" 
       and "(k\<^sub>1, p\<^sub>1)\<in> set t" "(k\<^sub>2, p\<^sub>2)\<in> set t"
     shows "k\<^sub>1 = k\<^sub>2 \<longleftrightarrow> p\<^sub>1 = p\<^sub>2"
-using assms proof(induction t arbitrary: k\<^sub>1 p\<^sub>1 k\<^sub>2 p\<^sub>2)
-  case (Node l k p r)
-  then show ?case
-  proof(cases "p\<^sub>1 = p")
-    case True
-    then show ?thesis sorry
-  next
-    case False
-    then show ?thesis sorry
-  qed
-qed(simp)
+proof
+  show "k\<^sub>1 = k\<^sub>2 \<Longrightarrow> p\<^sub>1 = p\<^sub>2"
+  using assms proof(induction t arbitrary: k\<^sub>1 p\<^sub>1 k\<^sub>2 p\<^sub>2)
+    case (Node l k p r)
+    then show ?case
+    using assms proof(cases "p\<^sub>1 = p\<^sub>2")
+      case False
+      then show "k\<^sub>1 = k\<^sub>2 \<Longrightarrow> p\<^sub>1 = p\<^sub>2" using assms sorry
+    qed(simp)
+  qed(simp)
+next
+  show "p\<^sub>1 = p\<^sub>2 \<Longrightarrow> k\<^sub>1 = k\<^sub>2" sorry
+  oops
 
 inductive is_bst :: "('a::linorder) treap \<Rightarrow> bool" where
   Leaf: "is_bst \<langle>\<rangle>" |
   Node: "\<lbrakk> is_bst l; is_bst r;
-        \<forall>(x\<^sub>k, x\<^sub>p) \<in> set l . x\<^sub>k < k; \<forall>(x\<^sub>k, x\<^sub>p) \<in> set r . k < x\<^sub>k \<rbrakk>
+        \<forall>(x\<^sub>k, x\<^sub>p) \<in> set l. x\<^sub>k < k; \<forall>(x\<^sub>k, x\<^sub>p) \<in> set r. k < x\<^sub>k \<rbrakk>
         \<Longrightarrow> is_bst \<langle>l, k, p, r\<rangle>"
+
+thm is_bst.induct
+lemma bst_rev:
+  "is_bst \<langle>l, k, p, r\<rangle> \<Longrightarrow> is_bst l \<and> is_bst r \<and> (\<forall>(x\<^sub>k, x\<^sub>p) \<in> set l . x\<^sub>k < k) \<and> (\<forall>(x\<^sub>k, x\<^sub>p) \<in> set r . k < x\<^sub>k)"
+  by(induction "\<langle>l, k, p, r\<rangle>" rule: is_bst.induct, blast)
+
+lemma smaller_key_is_left_child:
+  assumes "is_bst t"
+and "is_distinct t"
+  and "(k, d) \<in> set t"
+shows "k < key t \<Longrightarrow> (k, d) \<in> set (left t)"
+  using assms by(induction t arbitrary: k d rule: is_bst.induct, auto)
+
+lemma larger_key_is_right_child:
+  assumes "is_bst t"
+and "is_distinct t"
+  and "(k, d) \<in> set t"
+shows "key t < k \<Longrightarrow> (k, d) \<in> set (right t)"
+  using assms by(induction t arbitrary: k d rule: is_bst.induct, auto)
 
 inductive is_heap :: "('a::linorder) treap \<Rightarrow> bool" where
   Leaf: "is_heap \<langle>\<rangle>" |
@@ -202,10 +243,10 @@ proof
   then show "t = \<langle>\<rangle>" by(cases t, auto)
 qed(simp)
 
-lemma treap_is_unique:
+theorem treap_is_unique:
   assumes distinct:      "is_distinct t\<^sub>1" "is_distinct t\<^sub>2"
       and treaps:        "is_treap t\<^sub>1" "is_treap t\<^sub>2"
-      and equal_entries: "set t\<^sub>1 = set t\<^sub>2"
+      and equal_entries[simp]: "set t\<^sub>1 = set t\<^sub>2"
     shows "t\<^sub>1 = t\<^sub>2"
 using assms proof(induction t\<^sub>1 arbitrary: t\<^sub>2 rule:treap.induct)
   case Leaf
@@ -226,7 +267,8 @@ next
   let ?t\<^sub>2 = "\<langle>l\<^sub>2, k\<^sub>2, p\<^sub>2, r\<^sub>2\<rangle>"
   have "is_treap l\<^sub>2" "is_treap r\<^sub>2"
     using Node.prems(4) is_heap.cases is_bst.cases is_treap_def t2_def by fastforce+
-  
+
+  (* roots eq *)
   have "\<forall>(k', p') \<in> set (left ?t\<^sub>1) \<union> set (right ?t\<^sub>1). prio ?t\<^sub>1 < p'"
     using Node.prems(1, 3) heap_root_has_smallest_prio is_treap_def by blast
   then have "\<forall>(k', p') \<in> ?entries - {(k\<^sub>1, p\<^sub>1)}. prio ?t\<^sub>1 < p'"
@@ -236,18 +278,76 @@ next
   then have "\<forall>(k', p') \<in> set ?t\<^sub>1. prio ?t\<^sub>1 \<le> p'" by auto
   moreover have "\<forall>(k', p') \<in> set (left ?t\<^sub>2) \<union> set (right ?t\<^sub>2). prio ?t\<^sub>2 < p'"
     using Node.prems(2, 4) heap_root_has_smallest_prio is_treap_def t2_def by blast
-  then have "\<forall>(k', p') \<in> set ?t\<^sub>2 - {(k\<^sub>2, p\<^sub>2)}. prio ?t\<^sub>2 < p'"
+  then have root2_smallest_prio: "\<forall>(k', p') \<in> set ?t\<^sub>2 - {(k\<^sub>2, p\<^sub>2)}. prio ?t\<^sub>2 < p'"
     by simp
   then have "\<forall>(k', p') \<in> set ?t\<^sub>2 - {(k\<^sub>2, p\<^sub>2)}. prio ?t\<^sub>2 \<le> p'"
     using less_imp_le by blast
   then have "\<forall>(k', p') \<in> ?entries. prio ?t\<^sub>2 \<le> p'"
     using Node.prems(5) t2_def by auto
-  ultimately have equal_prio:  "p\<^sub>1 = p\<^sub>2"  sorry
-  have ""
-  then have "k\<^sub>1 = k\<^sub>2" using Node.prems(1, 2) sorry
-  have "\<forall>(k, p) \<in> ((set t\<^sub>2)-{(k\<^sub>2, p\<^sub>2)}). p\<^sub>2 < p" sorry
-  have "set l\<^sub>1 = set l\<^sub>2" sorry
-  with Node show ?case sorry
+  moreover have root1_in_set: "(k\<^sub>1, p\<^sub>1) \<in> ?entries"
+    by force
+  moreover have root2_in_set: "(k\<^sub>2, p\<^sub>2) \<in> ?entries"
+    using Node.prems(5) t2_def by auto
+  ultimately have equal_prio:  "prio ?t\<^sub>1 = prio ?t\<^sub>2"
+    by fastforce
+  then have roots_eq_prios: "p\<^sub>1 = p\<^sub>2" by simp
+  then have roots_eq_keys: "k\<^sub>1 = k\<^sub>2"
+    using Node.prems(5) case_prodD root1_in_set root2_smallest_prio t2_def by fastforce
+
+  (* left subtree eq *)
+  have "\<forall>(k', p') \<in> ?entries. k' < key ?t\<^sub>1 \<longrightarrow> (k', p') \<in> set (left ?t\<^sub>1)"
+    using Node.prems(1,3) is_treap_def smaller_key_is_left_child by fastforce
+  moreover have "\<forall>(k', p') \<in> ?entries.  \<not>k' < key ?t\<^sub>1 \<longrightarrow> (k', p') \<notin> set (left ?t\<^sub>1)"
+    using Node.prems(3) bst_rev is_treap_def by force
+  moreover have "set (left ?t\<^sub>1) \<subseteq> ?entries"
+    by auto
+  ultimately have left1: "{(k', p') \<in> ?entries. k' < key ?t\<^sub>1} = set (left ?t\<^sub>1)"
+    by blast
+
+  have "\<forall>(k', p') \<in> ?entries. k' < key ?t\<^sub>2 \<longrightarrow> (k', p') \<in> set (left ?t\<^sub>2)"
+    using Node.prems(2,4,5) is_treap_def smaller_key_is_left_child t2_def by fastforce
+  moreover have "\<forall>(k', p') \<in> ?entries.  \<not>k' < key ?t\<^sub>2 \<longrightarrow> (k', p') \<notin> set (left ?t\<^sub>2)"
+    using Node.prems(4) bst_rev is_treap_def t2_def
+    by (metis (no_types, lifting) case_prodD case_prodI2 key.simps(1) left.simps(1))
+  moreover have "set (left ?t\<^sub>2) \<subseteq> ?entries"
+    using Node.prems(5) t2_def by auto
+  ultimately have left2: "{(k', p') \<in> ?entries. k' < key ?t\<^sub>2} = set (left ?t\<^sub>2)"
+    by blast
+
+  from left1 left2 have "set (left ?t\<^sub>1) = set (left ?t\<^sub>2)"
+    by (simp add: roots_eq_keys)
+  then have left_subtrees_eq: "l\<^sub>1 = l\<^sub>2"
+    using Node.IH(1) \<open>is_treap l\<^sub>2\<close> Node.prems distinct_rev bst_rev is_heap.cases is_treap_def t2_def
+    by (metis left.simps(1) treap.distinct(1))
+
+  (* right subtree eq *)
+  have "\<forall>(k', p') \<in> ?entries. key ?t\<^sub>1 < k' \<longrightarrow> (k', p') \<in> set (right ?t\<^sub>1)"
+    using Node.prems(1,3) is_treap_def larger_key_is_right_child by fastforce
+  moreover have "\<forall>(k', p') \<in> ?entries.  \<not>key ?t\<^sub>1 < k' \<longrightarrow> (k', p') \<notin> set (right ?t\<^sub>1)"
+    using Node.prems(3) bst_rev is_treap_def by force
+  moreover have "set (right ?t\<^sub>1) \<subseteq> ?entries"
+    by auto
+  ultimately have right1: "{(k', p') \<in> ?entries. key ?t\<^sub>1 < k'} = set (right ?t\<^sub>1)"
+    by blast
+
+  have "\<forall>(k', p') \<in> ?entries.  key ?t\<^sub>2 < k' \<longrightarrow> (k', p') \<in> set (right ?t\<^sub>2)"
+    using Node.prems(2,4,5) is_treap_def larger_key_is_right_child t2_def by fastforce
+  moreover have "\<forall>(k', p') \<in> ?entries.  \<not>key ?t\<^sub>2 < k' \<longrightarrow> (k', p') \<notin> set (right ?t\<^sub>2)"
+    using Node.prems(4) bst_rev is_treap_def t2_def
+    by (metis (no_types, lifting) case_prodD case_prodI2 key.simps(1) right.simps(1))
+  moreover have "set (right ?t\<^sub>2) \<subseteq> ?entries"
+    using Node.prems(5) t2_def by auto
+  ultimately have right2: "{(k', p') \<in> ?entries. key ?t\<^sub>2 < k'} = set (right ?t\<^sub>2)"
+    by blast
+
+  from right1 right2 have "set (right ?t\<^sub>1) = set (right ?t\<^sub>2)"
+    by (simp add: roots_eq_keys)
+  then have right_subtrees_eq: "r\<^sub>1 = r\<^sub>2"
+    using Node.IH(2) \<open>is_treap r\<^sub>2\<close> Node.prems distinct_rev bst_rev is_heap.cases is_treap_def t2_def
+    by (metis right.simps(1) treap.distinct(1))
+
+  from left_subtrees_eq right_subtrees_eq show ?case
+    by (simp add: roots_eq_keys roots_eq_prios t2_def)
 qed
 
 end
